snap

io/Compile.ILang.To.RILang.fst
@@ -3,11 +3,10 @@ module Compile.ILang.To.RILang
 open FStar.Tactics
 open FStar.Tactics.Typeclasses
 
-open Common
+open IO.Sig
 open TC.Monitorable.Hist
 
-open Compile.ILang
-open Compile.RILang
+open Compiler.Languages
 
 class is_reifiable (reify_in:Type u#a) (pi:monitorable_prop) = {
   [@@@no_method]
@@ -36,6 +35,16 @@ class is_reflectable (reflect_out:Type u#a) (pi:monitorable_prop) = {
 
 #set-options "--print_implicits"
 
+instance reify_resexn pi (t1:Type) {| d1:is_reifiable t1 pi |} : is_reifiable (resexn t1) pi = {
+  ilang_reify_in = ilang_resexn pi t1 #d1.ilang_reify_in;
+  reify_out = resexn d1.reify_out;
+  rilang_reify_out = rilang_resexn pi d1.reify_out #d1.rilang_reify_out;
+  _reify = (fun r ->
+    match r with
+    | Inl x -> Inl (d1._reify x)
+    | Inr err -> Inr err)
+}
+
 instance reify_ilang_arrow
   pi
   (t1:Type) {| d1:is_reflectable t1 pi |} 
@@ -50,14 +59,14 @@ instance reify_ilang_arrow
     _reify = (fun (src_f:t1 -> IIOpi t2 pi) (tgt_x:d1.reflect_in) -> 
       let src_x : t1 = d1._reflect tgt_x in
       let src_f' : unit -> IIOpi t2 pi = (fun () -> src_f src_x) in
-      let tgt_f : IIO.dm_iio t2 (pi_as_hist pi) = IIO.__reify_IIOwp src_f' in
+      let tgt_f : dm_iio t2 (pi_as_hist pi) = __reify_IIOwp src_f' in
       
       (* these are just casts *)
-      let k : t2 -> IIO.dm_iio d2.reify_out (pi_as_hist pi) = (fun r -> IIO.dm_iio_return _ (d2._reify r)) in
+      let k : t2 -> dm_iio d2.reify_out (pi_as_hist pi) = (fun r -> dm_iio_return _ (d2._reify r)) in
       let wp : IO.Sig.hist d2.reify_out = Hist.hist_bind (pi_as_hist #t2 pi) (fun _ -> pi_as_hist pi) in 
-      let tgt_w : IIO.dm_iio d2.reify_out wp = IIO.dm_iio_bind _ _ _ _ tgt_f k in
+      let tgt_w : dm_iio d2.reify_out wp = dm_iio_bind _ _ _ _ tgt_f k in
       lemma_bind_pi_implies_pi #t2 #d2.reify_out pi;
-      let tgt_w : IIO.dm_iio d2.reify_out (pi_as_hist pi) = IIO.dm_iio_subcomp _ _ _ tgt_w in
+      let tgt_w : dm_iio d2.reify_out (pi_as_hist pi) = dm_iio_subcomp _ _ _ tgt_w in
       as_rilang_dm tgt_w
     );
   }
@@ -78,13 +87,13 @@ instance reflect_ilang_arrow
     let tree_f' : IO.Sig.iio d2.reflect_in = tree_f in
 
     (* these are just casts *)
-    assert (pi_as_hist pi `Hist.hist_ord` IIO.dm_iio_theta tree_f');
-    let tree_f : IIO.dm_iio d2.reflect_in (pi_as_hist pi) = tree_f' in
-    let k : d2.reflect_in -> IIO.dm_iio t2 (pi_as_hist pi) = (fun r -> IIO.dm_iio_return _ (d2._reflect r)) in
+    assert (pi_as_hist pi `Hist.hist_ord` dm_iio_theta tree_f');
+    let tree_f : dm_iio d2.reflect_in (pi_as_hist pi) = tree_f' in
+    let k : d2.reflect_in -> dm_iio t2 (pi_as_hist pi) = (fun r -> dm_iio_return _ (d2._reflect r)) in
     let wp : IO.Sig.hist t2 = Hist.hist_bind (pi_as_hist #d2.reflect_in pi) (fun _ -> pi_as_hist pi) in 
-    let tree_w : IIO.dm_iio t2 wp = IIO.dm_iio_bind _ _ _ _ tree_f k in
+    let tree_w : dm_iio t2 wp = dm_iio_bind _ _ _ _ tree_f k in
     lemma_bind_pi_implies_pi #d2.reflect_in #t2 pi;
-    let tree_w : IIO.dm_iio t2 (pi_as_hist pi) = IIO.dm_iio_subcomp _ _ _ tree_w in
-    IIO.IIOwp?.reflect tree_w) <: IIOpi t2 pi
+    let tree_w : dm_iio t2 (pi_as_hist pi) = dm_iio_subcomp _ _ _ tree_w in
+    IIOwp?.reflect tree_w) <: IIOpi t2 pi
   )
 }
