io/Compiler.Model.fst
@@ -1,5 +1,6 @@
 module Compiler.Model
 
+open FStar.Ghost
 open FStar.Tactics
 open FStar.Tactics.Typeclasses
 
@@ -9,68 +10,67 @@ open IO.Sig
 open TC.Monitorable.Hist
   
 open Compiler.Languages
-
 open Compile.IIO.To.ILang
 
+(** *** IIO interface **)
 noeq
-type iio_lang_interface = {
-  ct : Type;
+type iio_interface = {
+  ct : erased tflag -> Type;
   pt : Type;
 
-  vpi : monitorable_prop;
+  ct_rc : tree pck_rc;
+  pt_rc : tree pck_rc;
 
-  c1 : exportable pt vpi;
-  c2 : importable ct vpi;
+  ipi : monitorable_prop;
+
+  pt_exportable : fl:erased tflag -> exportable pt ipi pt_rc fl;
+  ct_importable : fl:erased tflag -> importable (ct fl) ipi ct_rc fl;
 }
 
-let test_interface : iio_lang_interface = {
-  pt = unit -> IIO unit (fun h -> True) (fun h r lt -> True);
-  ct = (x:file_descr) -> IIO unit (fun h -> is_open x h) (fun h r lt -> is_open x (apply_changes h lt));
+let make_all_rc_eff (i:iio_interface) : typ_posts AllActions i.ct_rc =
+  let r : tree (pck_eff_rc AllActions) = map_tree i.ct_rc make_rc_eff in
+  assume (equal_trees i.ct_rc (map_tree r dfst));
+  r
 
-  vpi = (fun _ _ _ -> true);
+type ctx_iio (i:iio_interface) = #fl:erased tflag -> typ_posts fl i.ct_rc -> i.ct fl 
 
-  c1 = admit ();
-  c2 = admit ();
-}
+type prog_iio (i:iio_interface) = i.ct AllActions -> i.pt
 
-type iio_lang_ctx (i:iio_lang_interface) = i.ct
-type iio_lang_prog (i:iio_lang_interface) = iio_lang_ctx i -> i.pt
+let iio_language : language = {
+  interface = iio_interface;
 
-let iio_lang_language : language = {
-  interface = iio_lang_interface;
+  ctx = ctx_iio;
+  pprog = prog_iio;
+  whole = (i:iio_interface & i.pt);
 
-  ctx = iio_lang_ctx;
-  pprog = iio_lang_prog;
-  whole = (i:iio_lang_interface & i.pt);
-
-  link = (fun #i p c -> (| i, p c |));
+  link = (fun #i p c -> 
+    let eff_rc = make_all_rc_eff i in
+    (| i, p (c #AllActions eff_rc) |));
   event_typ = IO.Sig.event;
 
   beh = admit ()
 }
 
-val test_prog : iio_lang_prog test_interface
-let test_prog ctx () =
-  let fd = static_cmd Openfile "../Makefile" in
-  if Inl? fd then ctx (Inl?.v fd)
-  else ()
-
+(** *** ILang interface **)
 noeq
 type ilang_interface = {
   pt : Type;
-  ct : Type;
+  ct : erased tflag -> Type;
 
-  vpi : monitorable_prop;
+  ipi : monitorable_prop;
+  
+  pt_ilang : ilang pt ipi;
+  ct_ilang : fl:erased tflag -> ilang (ct fl) ipi;
 }
 
-type ilang_ctx (i:ilang_interface) = i.ct
-type ilang_prog (i:ilang_interface) = ilang_ctx i -> i.pt
+type ctx_ilang (i:ilang_interface) = #fl:erased tflag -> i.ct fl
+type prog_ilang (i:ilang_interface) = i.ct AllActions -> i.pt
 
 let ilang_language : language = {
   interface = ilang_interface;
 
-  ctx = ilang_ctx;
-  pprog = ilang_prog;
+  ctx = ctx_ilang;
+  pprog = prog_ilang;
   whole = (i:ilang_interface & i.pt);
 
   link = (fun #i p c -> (| i, p c |));
@@ -79,17 +79,99 @@ let ilang_language : language = {
   beh = admit ();
 }
 
-let comp_int (i:iio_lang_interface) : ilang_interface = {
-    pt = resexn i.c1.etype;
-    ct = i.c2.itype;
-    vpi = i.vpi;
+(** *** RILang interface **)
+noeq
+type rilang_interface = {
+  pt : Type;
+  ct : Type;
+
+  ipi : monitorable_prop;
+  
+  pt_rilang : rilang pt ipi;
+  ct_rilang : rilang ct ipi;
 }
 
-let compiler_pprog (#i:iio_lang_interface) (p:iio_lang_language.pprog i) : ilang_language.pprog (comp_int i) = fun c -> 
-    match i.c2.import c with
-    | Inl c' -> begin 
-      let (| _, pt |) = iio_lang_language.link #i p c' in
-      Inl (i.c1.export pt)
+type rilang_ctx (i:rilang_interface) = i.ct
+type rilang_prog (i:rilang_interface) = rilang_ctx i -> i.pt
+
+let rilang_language : language = {
+  interface = rilang_interface;
+
+  ctx = rilang_ctx;
+  pprog = rilang_prog;
+  whole = (i:rilang_interface & i.pt);
+
+  link = (fun #i p c -> (| i, p c |));
+  event_typ = IO.Sig.event;
+
+  beh = admit ();
+}
+
+(** *** TLang interface **)
+noeq
+type tlang_interface = {
+  pt : Type u#a;
+  ct : (Type u#b ->Type u#(max 1 b))->Type;
+
+  ipi : monitorable_prop;
+  
+  pt_rilang : rilang pt ipi;
+  ct_rilang : rilang (ct (dm_mon ipi).m) ipi;
+}
+
+type tlang_ctx (i:tlang_interface) = mon:monad -> acts mon -> i.ct mon.m
+type tlang_prog (i:tlang_interface) = i.ct ((dm_mon i.ipi).m) -> i.pt
+
+let tlang_language : language = {
+  interface = tlang_interface;
+
+  ctx = tlang_ctx;
+  pprog = tlang_prog;
+  whole = (i:tlang_interface & i.pt);
+
+  link = (fun #i p c -> (| i, p (c (dm_mon i.ipi) (dm_acts i.ipi)) |));
+  event_typ = IO.Sig.event;
+
+  beh = admit ();
+}
+
+(** ** Compile interfaces **)
+let comp_int_iio_ilang (i:iio_lang_interface) : ilang_interface = {
+    pt = resexn i.pt_exportable.etype;
+    ct = i.ct_importable.itype;
+    ipi = i.ipi;
+
+    pt_ilang = ilang_resexn i.ipi i.pt_exportable.etype #i.pt_exportable.c_etype;
+    ct_ilang = i.ct_importable.c_itype;
+
+    pt_reifiable = reify_resexn i.ipi i.pt_exportable.etype #i.pt_reifiable;
+    ct_reflectable = i.ct_reflectable; 
+}
+
+let comp_int_ilang_rilang (i:ilang_interface) : rilang_interface = {
+    pt = i.pt_reifiable.reify_out;
+    ct = i.ct_reflectable.reflect_in;
+    ipi = i.ipi;
+
+    pt_rilang = i.pt_reifiable.rilang_reify_out;
+    ct_rilang = i.ct_reflectable.rilang_reflect_in;
+}
+
+let comp_int_rilang_tlang (i:rilang_interface) : tlang_interface = {
+    pt = i.pt;
+    ct = (fun m -> i.ct); // is this ok?
+    ipi = i.ipi;
+
+    pt_rilang = i.pt_rilang;
+    ct_rilang = i.ct_rilang; // I suppose yes because of this constraint
+}
+
+(** ** Phases of compilation **)
+let compiler_pprog_iio_ilang (#i:iio_lang_interface) (p_s:iio_lang_language.pprog i) : ilang_language.pprog (comp_int_iio_ilang i) = fun c_t -> 
+    match i.ct_importable.import c_t with
+    | Inl c_s -> begin 
+      let (| _, ws |) = iio_lang_language.link #i p_s c_s in
+      Inl (i.pt_exportable.export ws)
     end
     | Inr err -> Inr err
 
@@ -97,10 +179,59 @@ let phase1 : compiler = {
   source = iio_lang_language;
   target = ilang_language;
 
-  comp_int = comp_int;
+  comp_int = comp_int_iio_ilang;
 
-  compile_pprog = compiler_pprog;
+  compile_pprog = compiler_pprog_iio_ilang;
 
-  rel_traces = admit ();
+  rel_traces = (==);
 }
 
+let compiler_pprog_ilang_rilang (#i:ilang_interface) (p_s:ilang_language.pprog i) : rilang_language.pprog (comp_int_ilang_rilang i) = fun c_t -> 
+  let c_s = i.ct_reflectable._reflect c_t in
+  let (| _, ws |) = ilang_language.link #i p_s c_s in
+  i.pt_reifiable._reify ws
+
+let phase2 : compiler = {
+  source = ilang_language;
+  target = rilang_language;
+
+  comp_int = comp_int_ilang_rilang;
+
+  compile_pprog = compiler_pprog_ilang_rilang;
+
+  rel_traces = (==);
+}
+
+let compiler_pprog_rilang_tlang (#i:rilang_interface) (p_s:rilang_language.pprog i) : tlang_language.pprog (comp_int_rilang_tlang i) = p_s
+
+let phase3 : compiler = {
+  source = rilang_language;
+  target = tlang_language;
+
+  comp_int = comp_int_rilang_tlang;
+
+  compile_pprog = compiler_pprog_rilang_tlang;
+
+  rel_traces = (==);
+}
+
+let compiler = (phase1 `chain_compilers` phase2) `chain_compilers` phase3
+
+(** Tests **)
+let test_interface : iio_lang_interface = {
+  pt = unit -> IIO unit (fun h -> True) (fun h r lt -> True);
+  ct = (x:file_descr) -> IIO unit (fun h -> is_open x h) (fun h r lt -> is_open x (apply_changes h lt));
+
+  ipi = (fun _ _ _ -> true);
+
+  pt_exportable = admit ();
+  ct_importable = admit ();
+  pt_reifiable = admit ();
+  ct_reflectable = admit ();
+}
+
+val test_prog : iio_lang_prog test_interface
+let test_prog ctx () =
+  let fd = static_cmd Openfile "../Makefile" in
+  if Inl? fd then ctx (Inl?.v fd)
+  else ()
